src/FsTactics.v
@@ -23,3 +23,15 @@ Ltac inv_sig :=
   | [ H: sig _ |- _ ] => inversion H
   end.
 
+Ltac invert_rel R := repeat match goal with
+  | [ H: R _ _ |- _ ] => inversion H; clear H
+  end.
+
+Ltac generalize_all := repeat match goal with
+  | [ H: _ |- _ ] => generalize H; clear H
+  end.
+
+Ltac destruct_type T := repeat match goal with
+  | [ H: T |- _ ] => destruct H
+  end.
+
